Update Coq development

Common/Definitions.v
@@ -1,3 +1,12 @@
+Require Export Common.Maps.
+
+Require Export Coq.Bool.Bool.
+Require Export Coq.Lists.List.
+Require Export Coq.Arith.Arith.
+
+Export ListNotations.
+Open Scope list_scope.
+
 Module Procedure.
   Definition id := nat.
 End Procedure.
@@ -6,12 +15,41 @@ Module Component.
   Definition id := nat.
 
   Record interface := mkCompInterface {
-    name : id;
-    export : nat;
-    import : list (id * Procedure.id)
+    export : list Procedure.id;
+    import : list (Component.id * Procedure.id)
   }.
+
+  Definition is_importing CI C P : Prop := In (C,P) (import CI).
+  Definition is_exporting CI P : Prop := In P (export CI).
 End Component.
 
 Module Program.
-  Definition interface := list Component.interface.
+  Definition interface := NMap.t Component.interface.
+  Definition has_component Is C (CI : Component.interface) := NMap.MapsTo C CI Is.
 End Program.
+
+Definition exported_procedure
+           (Is : Program.interface)
+           (C : Component.id) (P : Procedure.id) :=
+  exists CI,
+    Program.has_component Is C CI /\ Component.is_exporting CI P.
+
+Definition imported_procedure
+           (Is : Program.interface)
+           (C C': Component.id) (P : Procedure.id) : Prop :=
+  exists CI,
+    Program.has_component Is C CI /\ Component.is_importing CI C' P.
+
+Lemma procs_eqdec (CP : Component.id * Procedure.id) (CP' : Component.id * Procedure.id) :
+  {CP=CP'} + {CP<>CP'}.
+Proof.
+  repeat decide equality.
+Qed.
+
+Definition imported_procedure_b
+           (Is : Program.interface)
+           (C C': Component.id) (P : Procedure.id) : bool :=
+  match NMap.find C Is with
+  | Some CI => negb ((count_occ procs_eqdec (Component.import CI) (C',P)) =? 0)
+  | None => false
+  end.
