Common/Util.v
@@ -1,72 +1,89 @@
-Require Export Coq.Lists.List.
-Require Export Coq.Bool.Bool.
-Require Export Coq.Arith.Arith.
-
-Export ListNotations.
-Open Scope list_scope.
-
-Definition admit {T: Type} : T. Admitted.
+Require Import Common.Definitions.
 
 Module Util.
-  Fixpoint mem x xs :=
-    match xs with
-    | [] => false
-    | x' :: xs' => if x =? x' then true else mem x xs'
-    end.
+  Module Nat.
+    Fixpoint safe_sub (n1 n2 : nat) : option nat :=
+      match n1, n2 with
+      | 0    , 0     => Some 0
+      | 0    , S _   => None (* underflow *)
+      | S _  , 0     => Some n1
+      | S n1', S n2' => safe_sub n1' n2'
+      end.
 
-  Lemma not_in_iff_mem_false :
-    forall x xs,
-      ~ (In x xs) <-> mem x xs = false.
-  Proof.
-    intros. split.
-    - intro Hxs. induction xs.
-      + auto.
-      + simpl.
-        apply not_in_cons in Hxs. destruct Hxs.
-        unfold not in H.
-        destruct (x =? a) eqn:Heq_xa.
-        * exfalso. apply beq_nat_true in Heq_xa.
-          apply H. apply Heq_xa.
-        * apply IHxs. apply H0.
-    - intro Hxs. induction xs.
-      + auto.
-      + destruct (x =? a) eqn:Heq_xa.
-        * apply not_in_cons.
-          split;
-            unfold mem in Hxs; rewrite Heq_xa in Hxs;
-              discriminate Hxs.
-        * apply not_in_cons. split.
-          ** intro Heq_xa_true.
-             rewrite Heq_xa_true in Heq_xa. simpl in Heq_xa.
-             apply beq_nat_false in Heq_xa. auto.
-          ** apply IHxs.
-             unfold mem in Hxs. rewrite Heq_xa in Hxs.
-             auto.
-  Qed.
+    Definition of_bool (b : bool) : nat :=
+      if b then 1 else 0.
+  End Nat.
 
-  Lemma in_iff_mem_true :
-    forall x xs,
-      In x xs <-> mem x xs = true.
-  Proof.
-    intros. split.
-    - intro Hxs.
-      induction xs.
-      + auto.
-      + simpl.
-        destruct (x =? a) eqn:Heq_xa.
-        * reflexivity.
-        * apply IHxs. apply in_inv in Hxs. destruct Hxs.
-          ** exfalso. rewrite beq_nat_false_iff in Heq_xa.
-             apply Heq_xa. symmetry. auto.
-          ** auto.
-    - intro Hxs.
-      induction xs.
-      + discriminate Hxs.
-      + simpl.
-        destruct (x =? a) eqn:Heq_xa.
-        * left. symmetry. apply beq_nat_true in Heq_xa. auto.
-        * right. apply IHxs.
-          unfold mem in Hxs.
-          rewrite Heq_xa in Hxs. auto.
-  Qed.
+  Module Lists.
+    Fixpoint update {A : Type} (l : list A) (n : nat) (val : A) {struct l} : list A :=
+      match l with
+      | [] => []
+      | x :: xs => match n with
+                   | 0 => val :: xs
+                   | S n' => x :: update xs n' val
+                   end
+      end.
+
+    Fixpoint mem x xs :=
+      match xs with
+      | [] => false
+      | x' :: xs' => if x =? x' then true else mem x xs'
+      end.
+
+    Lemma not_in_iff_mem_false :
+      forall x xs,
+        ~ (In x xs) <-> mem x xs = false.
+    Proof.
+      intros. split.
+      - intro Hxs. induction xs.
+        + auto.
+        + simpl.
+          apply not_in_cons in Hxs. destruct Hxs.
+          unfold not in H.
+          destruct (x =? a) eqn:Heq_xa.
+          * exfalso. apply beq_nat_true in Heq_xa.
+            apply H. apply Heq_xa.
+          * apply IHxs. apply H0.
+      - intro Hxs. induction xs.
+        + auto.
+        + destruct (x =? a) eqn:Heq_xa.
+          * apply not_in_cons.
+            split;
+              unfold mem in Hxs; rewrite Heq_xa in Hxs;
+                discriminate Hxs.
+          * apply not_in_cons. split.
+            ** intro Heq_xa_true.
+               rewrite Heq_xa_true in Heq_xa. simpl in Heq_xa.
+               apply beq_nat_false in Heq_xa. auto.
+            ** apply IHxs.
+               unfold mem in Hxs. rewrite Heq_xa in Hxs.
+               auto.
+    Qed.
+
+    Lemma in_iff_mem_true :
+      forall x xs,
+        In x xs <-> mem x xs = true.
+    Proof.
+      intros. split.
+      - intro Hxs.
+        induction xs.
+        + auto.
+        + simpl.
+          destruct (x =? a) eqn:Heq_xa.
+          * reflexivity.
+          * apply IHxs. apply in_inv in Hxs. destruct Hxs.
+            ** exfalso. rewrite beq_nat_false_iff in Heq_xa.
+               apply Heq_xa. symmetry. auto.
+            ** auto.
+      - intro Hxs.
+        induction xs.
+        + discriminate Hxs.
+        + simpl.
+          destruct (x =? a) eqn:Heq_xa.
+          * left. symmetry. apply beq_nat_true in Heq_xa. auto.
+          * right. apply IHxs.
+            unfold mem in Hxs.
+            rewrite Heq_xa in Hxs. auto.
+    Qed.
+  End Lists.
 End Util.
