Intermediate/CS.v
@@ -1,551 +1,109 @@
 Require Import Common.Definitions.
 Require Import Common.Util.
+Require Import Common.Linking.
 Require Import Common.Events.
 Require Import Common.Smallstep.
+Require Import Common.Memory.
 Require Import Intermediate.Machine.
+Require Import Intermediate.GlobalEnv.
 
 Module CS.
-  Import IntermediateMachine.
-  
-  Record program := {
-    prog_interface : Program.interface;
-    prog_memory : Memory.data;
-    prog_entrypoints : EntryPoint.data;
-    prog_entrypoints_wf :
-      forall CI C,
-        In CI prog_interface ->
-        Component.name CI = C ->
-        M.In C prog_entrypoints /\
-        exists addrs, M.MapsTo C addrs prog_entrypoints
-  }.
+  Import Intermediate.
 
-  Definition stack : Type := list (Component.id * Memory.address).
+  Definition stack : Type := list Pointer.t.
 
-  Definition state : Type := 
-    Component.id * stack * Memory.data * Register.data * Memory.address.
-
-  Definition comp_of_state (s : state) : Component.id :=
-    match s with (C,_,_,_,_) => C end.
-
-  Definition mem_of_state (s : state) : Memory.data :=
-    match s with (_,_,mem,_,_) => mem end.
-
-  Record global_env := mkGlobalEnv {
-    genv_interfaces : Program.interface;
-    genv_entrypoints : EntryPoint.data;
-  }.
-
-  Definition initial_state_for (p : program) : state :=
-    let mem := prog_memory p in
-    let E := prog_entrypoints p in
-    (0, [], mem, Register.empty, EntryPoint.get 0 0 E).
-
-  (* predicates on states *)
-
-  Definition initial_state p (s : state) : Prop :=
-    match s with (C, d, mem, regs, pc) =>
-      C = 0 /\ d = [] /\
-      regs = Register.empty /\
-      pc = EntryPoint.get 0 0 (prog_entrypoints p)
-    end.
-
-  Definition final_state (s : state) : Prop :=
-    match s with (C, d, mem, regs, pc) =>
-      executing Halt C mem pc
-    end.
-
-  Definition error_state (G : global_env) (s : state) : Prop :=
-    match s with (C, d, mem, regs, pc) =>
-      (* decoding error *)
-      EncDec.decode (Memory.get mem C pc) = None
-      (* call on the executing component *)
-      \/ (exists P,
-             executing (Call C P) C mem pc)
-      (* illegal call, we cannot check priviledges *)
-      \/ (exists C' P,
-             executing (Call C' P) C mem pc ->
-             let Is := genv_interfaces G in
-             find (fun C'' => C =? Component.name C'') Is = None)
-      (* illegal call to a not existing component *)
-      \/ (exists C' P,
-             executing (Call C' P) C mem pc ->
-             let Is := genv_interfaces G in
-             find (fun C'' => C' =? Component.name C'') Is = None)
-      (* illegal call to a not imported component *)
-      \/ (exists CI C' P,
-             executing (Call C' P) C mem pc ->
-             let Is := genv_interfaces G in
-             find (fun C'' => C =? Component.name C'') Is = Some CI ->
-             ~ (In (C',P) (Component.import CI)))
-      (* illegal call to a not exported procedure *)
-      \/ (exists C'I C' P,
-             executing (Call C' P) C mem pc ->
-             let Is := genv_interfaces G in
-             find (fun C'' => C' =? Component.name C'') Is = Some C'I ->
-             ~ (P < Component.export C'I))
-      (* return with empty stack *)
-      \/ (executing Return C mem pc -> d = [])
-      (* return on the executing component *)
-      \/ (exists addr (d' : stack),
-             executing Return C mem pc ->
-             d = (C, addr) :: d')
-    end.
-
- Definition undefined_behavior_state (G : global_env) (s : state) : Prop :=
-    match s with (C, d, mem, regs, pc) =>
-      (* load failure *)
-      (exists r1 r2,
-          executing (Load r1 r2) C mem pc ->
-          Memory.get mem C (Register.get r1 regs) = None)
-      (* write failure *)
-      \/ (exists r1 r2,
-             executing (Store r1 r2) C mem pc ->
-             Memory.set mem C (Register.get r1 regs) (Register.get r2 regs) = None)
-    end.
-
-  (* small-step semantics *)
-
-  Definition eval_binop (e : binop) (a b : nat) : nat :=
-    match e with
-    | Add   => a + b
-    | Minus => a - b
-    | Mul   => a * b
-    | Eq    => if a  =? b then 1 else 0
-    | Leq   => if a <=? b then 1 else 0
-    end.
-
-  Reserved Notation "G |-CS s1 '=>[' t ']' s2" (at level 40).
+  Definition state : Type := stack * Memory.t * Register.t * Pointer.t.
 
   Inductive step (G : global_env) : state -> trace -> state -> Prop :=
-  | Nop: forall mem C pc d regs,
-      executing Nop C mem pc ->
-      G |-CS (C,d,mem,regs,pc) =>[E0] (C,d,mem,regs,pc+1)
+  | Nop: forall gps mem regs pc,
+      executing G pc Nop ->
+      step G (gps, mem, regs, pc) E0 (gps, mem, regs, Pointer.inc pc)
 
-  | Const: forall mem C pc r cval d regs regs',
-      executing (Const cval r) C mem pc ->
-      regs' = Register.set r cval regs ->
-      G |-CS (C,d,mem,regs,pc) =>[E0] (C,d,mem,regs',pc+1)
+  | Const: forall gps mem regs regs' pc r v,
+      executing G pc (Const v r) ->
+      Register.set r (imm_to_val v) regs = regs' ->
+      step G (gps, mem, regs, pc) E0 (gps, mem, regs', Pointer.inc pc)
 
-  | Mov: forall mem C pc r1 r2 regs regs' d,
-      executing (Mov r1 r2) C mem pc ->
-      regs' = Register.set r2 (Register.get r1 regs) regs ->
-      G |-CS (C,d,mem,regs,pc) =>[E0] (C,d,mem,regs',pc+1)
+  | Mov: forall gps mem regs regs' pc r1 r2,
+      executing G pc (Mov r1 r2) ->
+      Register.set r2 (Register.get r1 regs) regs = regs' ->
+      step G (gps, mem, regs, pc) E0 (gps, mem, regs', Pointer.inc pc)
 
-  | BinOp: forall mem C pc r1 r1val r2 r2val r3 regs regs' d op,
-      executing (BinOp op r1 r2 r3) C mem pc ->
-      r1val = Register.get r1 regs ->
-      r2val = Register.get r2 regs ->
-      regs' = Register.set r3 (eval_binop op r1val r2val) regs ->
-      G |-CS (C,d,mem,regs,pc) =>[E0] (C,d,mem,regs',pc+1)
+  | BinOp: forall gps mem regs regs' pc r1 r2 r3 op,
+      executing G pc (BinOp op r1 r2 r3) ->
+      Register.set r3
+                   (eval_binop op (Register.get r1 regs) (Register.get r2 regs))
+                   regs = regs' ->
+      step G (gps, mem, regs, pc) E0 (gps, mem, regs', Pointer.inc pc)
 
-  | Load: forall mem C pc r1 r2 regs regs' d addr memval,
-      executing (Load r1 r2) C mem pc ->
-      addr = Register.get r1 regs ->
-      Some memval = Memory.get mem C addr ->
-      regs' = Register.set r2 memval regs ->
-      G |-CS (C,d,mem,regs,pc) =>[E0] (C,d,mem,regs',pc+1)
+  | Load: forall gps mem regs regs' pc r1 r2 ptr v,
+      executing G pc (Load r1 r2) ->
+      Register.get r1 regs = Ptr ptr ->
+      Memory.load mem ptr = Some v ->
+      Register.set r2 v regs = regs' ->
+      step G (gps, mem, regs, pc) E0 (gps, mem, regs', Pointer.inc pc)
 
-  | Store: forall mem C pc r1 r2 regs d addr value mem',
-      executing (Store r1 r2) C mem pc->
-      addr = Register.get r1 regs ->
-      value = Register.get r2 regs ->
-      Some mem' = Memory.set mem C addr value ->
-      G |-CS (C,d,mem,regs,pc) =>[E0] (C,d,mem',regs,pc+1)
+  | Store: forall gps mem regs pc ptr r1 r2 mem',
+      executing G pc (Store r1 r2) ->
+      Register.get r1 regs = Ptr ptr ->
+      Pointer.component ptr = Pointer.component pc ->
+      Memory.store mem ptr (Register.get r2 regs) = Some mem' ->
+      step G (gps, mem, regs, pc) E0 (gps, mem', regs, Pointer.inc pc)
 
-  | Jal: forall mem C pc val r regs regs' d,
-      executing (Jal r) C mem pc->
-      val = Register.get r regs ->
-      regs' = Register.set r (pc+1) regs ->
-      G |-CS (C,d,mem,regs,pc) =>[E0] (C,d,mem,regs',val)
+  | Jal: forall gps mem regs regs' pc pc' l,
+      executing G pc (Jal l) ->
+      find_label_in_component G pc l = Some pc' ->
+      Register.set R_RA (Ptr (Pointer.inc pc)) regs = regs' ->
+      step G (gps, mem, regs, pc) E0 (gps, mem, regs', pc')
 
-  | Jump: forall mem C pc addr r regs d,
-      executing (Jump r) C mem pc->
-      Register.get r regs = addr ->
-      G |-CS (C,d,mem,regs,pc) =>[E0] (C,d,mem,regs,addr)
+  | Jump: forall gps mem regs pc pc' r,
+      executing G pc (Jump r) ->
+      Register.get r regs = Ptr pc' ->
+      Pointer.component pc' = Pointer.component pc ->
+      step G (gps, mem, regs, pc) E0 (gps, mem, regs, pc')
 
-  | BnzNZ: forall mem C pc offset r regs d,
-      executing (Bnz r offset) C mem pc ->
-      Register.get r regs <> 0 ->
-      G |-CS (C,d,mem,regs,pc) =>[E0] (C,d,mem,regs,pc+offset)
+  | BnzNZ: forall gps mem regs pc pc' r l val,
+      executing G pc (Bnz r l) ->
+      Register.get r regs = Int val ->
+      val <> 0 ->
+      find_label_in_procedure G pc l = Some pc' ->
+      step G (gps, mem, regs, pc) E0 (gps, mem, regs, pc')
 
-  | BnzZ: forall mem C pc offset r regs d,
-      executing (Bnz r offset) C mem pc ->
-      Register.get r regs = 0 ->
-      G |-CS (C,d,mem,regs,pc) =>[E0] (C,d,mem,regs,pc+1)
+  | BnzZ: forall gps mem regs pc pc' r l,
+      executing G pc (Bnz r l) ->
+      Register.get r regs = Int 0 ->
+      find_label_in_procedure G pc l = Some pc' ->
+      step G (gps, mem, regs, pc) E0 (gps, mem, regs, pc')
 
-  | Call: forall mem C pc regs d d' C' P,
-      executing (Call C' P) C mem pc ->
-      call_is_public_and_exists (genv_interfaces G) C' P ->
-      call_is_in_imports (genv_interfaces G) C C' P ->
-      C' <> C ->
-      d' = (C,pc+1) :: d ->
-      let t := [ECall C P (Register.get Register.R_COM regs) C'] in
-      let E := genv_entrypoints G in
-      G |-CS (C,d,mem,regs,pc) =>[t]
-             (C',d',mem,regs,EntryPoint.get C' P E)
+  | Alloc: forall gps mem mem' regs regs' pc rsize rptr size ptr,
+      executing G pc (Alloc rptr rsize) ->
+      Register.get rsize regs = Int size ->
+      Memory.alloc mem (Pointer.component pc) size = Some (mem', ptr) ->
+      Register.set rptr (Ptr ptr) regs = regs' ->
+      step G (gps, mem, regs, pc) E0 (gps, mem', regs', Pointer.inc pc)
 
-  | Return: forall mem C pc pc' d' regs d C',
-      executing Return C mem pc ->
-      d = (C',pc') :: d' ->
-      C <> C' ->
-      let t := [ERet C (Register.get Register.R_COM regs) C'] in
-      G |-CS (C,d,mem,regs,pc) =>[t] (C',d',mem,regs,pc')
+  | Call: forall gps gps' mem regs pc b C' P rcomval,
+      executing G pc (Call C' P) ->
+      Pointer.component pc <> C' ->
+      imported_procedure (genv_interface G) (Pointer.component pc) C' P ->
+      gps' = Pointer.inc pc :: gps ->
+      EntryPoint.get C' P (genv_entrypoints G) = Some b ->
+      let pc' := (C', b, 0) in
+      Register.get R_COM regs = Int rcomval ->
+      let t := [ECall (Pointer.component pc) P rcomval C'] in
+      step G (gps, mem, regs, pc) t (gps', mem, Register.invalidate regs, pc')
 
-  where "G |-CS s1 '=>[' t ']' s2" := (step G s1 t s2).
+  | Return: forall gps gps' mem regs pc pc' rcomval,
+      executing G pc Return ->
+      gps = pc' :: gps' ->
+      Pointer.component pc <> Pointer.component pc' ->
+      Register.get R_COM regs = Int rcomval ->
+      let t := [ERet (Pointer.component pc) rcomval (Pointer.component pc')] in
+      step G (gps, mem, regs, pc) t (gps', mem, Register.invalidate regs, pc').
 
-  (* complete program semantics *)
-
-  Section SEMANTICS.
-    Variable p : program.
-
-    Definition semantics :=
-      @Semantics_gen state global_env
-                     step
-                     (initial_state p)
-                     final_state
-                     (mkGlobalEnv (prog_interface p) (prog_entrypoints p)).
-  End SEMANTICS.
-
-  (* sanity checks *)
-
-  Theorem states_characterization:
-    forall G s,
-      (exists t s', G |-CS s =>[t] s') \/
-      final_state s \/
-      error_state G s \/
-      undefined_behavior_state G s.
-  Proof.
-    intros G s.
-    destruct s as [[[[C d] mem] regs] pc].
-    (* can we take a step? *)
-    destruct (EncDec.decode (Memory.get mem C pc))
-      as [instr | ?] eqn:Hdecode.
-    (* case analysis on the current instruction *)
-    - destruct instr.
-      (* NOP *)
-      + left. eexists. eexists. eapply Nop. auto.
-      (* CONST *)
-      + left. eexists.
-        exists (C,d,mem,Register.set r n regs,pc+1).
-        eapply Const; eauto.
-      (* MOV *)
-      + left. eexists.
-        exists (C,d,mem,Register.set r0 (Register.get r regs) regs,pc+1).
-        eapply Mov; eauto.
-      (* BINOP *)
-      + left. eexists.
-        exists (C,d,mem,
-                Register.set
-                  r1 (eval_binop b (Register.get r regs) (Register.get r0 regs)) regs,
-                pc+1).
-        eapply BinOp; eauto.
-      (* LOAD *)
-      + (* check whether the load succeeds *)
-        destruct (Memory.get mem C (Register.get r regs))
-          as [memval | ?] eqn:Hload_result.
-        (* SUCCESS *)
-        * left. exists E0.
-          exists (C,d,mem,Register.set r0 memval regs,pc+1).
-          eapply Load; eauto.
-        (* INVALID COMPONENT
-           NOTE: with the new memory model there
-                 will also be OUT OF BOUND *)
-        * unfold undefined_behavior_state.
-          right. right. right. left. exists r, r0. intros. auto.
-      (* STORE *)
-      + (* check whether the write succeeds *)
-        destruct (Memory.set mem C (Register.get r regs) (Register.get r0 regs))
-          as [mem' | ?] eqn:Hwrite_result.
-        (* SUCCESS *)
-        * left. exists E0.
-          exists (C,d,mem',regs,pc+1).
-          eapply Store; eauto.
-        (* INVALID COMPONENT
-           NOTE: with the new memory model there
-                 will also be OUT OF BOUND *)
-        * unfold undefined_behavior_state.
-          right. right. right. right. exists r, r0.
-          intros. auto. 
-      (* BNZ *)
-      + destruct (Register.get r regs =? 0) eqn:Hbranch;
-          left; eexists; eexists.
-        (* register is zero *)
-        * rewrite beq_nat_true_iff in Hbranch.
-          eapply BnzZ; eauto.
-        (* register is not zero *)
-        * rewrite beq_nat_false_iff in Hbranch.
-          eapply BnzNZ; eauto.
-      (* JUMP *)
-      + left. eexists. exists (C,d,mem,regs,Register.get r regs).
-        eapply Jump; eauto.
-      (* JAL *)
-      + left. eexists.
-        exists (C,d,mem,Register.set r (pc+1) regs,Register.get r regs).
-        eapply Jal; eauto.
-      (* CALL *)
-      + remember i as C'.
-        remember i0 as P.
-        destruct (C' =? C) eqn:Hcall_target.
-        (* ERROR, call to the same component *)
-        * unfold error_state.
-          rewrite beq_nat_true_iff in Hcall_target.
-          rewrite <- Hcall_target.
-          eauto 7.
-        * (* does the current component has an interface? *)
-          destruct (find (fun C'' => C =? Component.name C'') (genv_interfaces G))
-            as [CI | ?] eqn:Hcur_comp_existence.
-          ** (* does the target component exist? *)
-             rewrite beq_nat_false_iff in Hcall_target.
-             destruct (find (fun C'' => C' =? Component.name C'') (genv_interfaces G))
-               as [C'I | ?] eqn:Htarget_existence.
-             *** (* can the component call the specified target? *)
-                 destruct (find (fun entry =>
-                                   match entry with
-                                   | (C'',P') => andb (C'' =? C') (P' =? P)
-                                   end) (Component.import CI))
-                   as [[C'' P'] | ?] eqn:Hcomponent_import.
-                 **** destruct (find_some
-                                  (fun entry : nat * nat =>
-                                     let (C'', P') := entry in (C'' =? C') && (P' =? P))
-                                  _  Hcomponent_import) as [Hin_import Hcomp_names].
-                      unfold andb in Hcomp_names.
-                      assert (HC''C': C'' = C'). {
-                        destruct (C'' =? C') eqn:HC''C'.
-                        + apply beq_nat_true_iff in HC''C'. auto.
-                        + inversion Hcomp_names.
-                      }
-                      rewrite HC''C' in Hcomp_names.
-                      rewrite <- beq_nat_refl in Hcomp_names.
-                      rewrite beq_nat_true_iff in Hcomp_names.
-                      (* is the target procedure exported? *)
-                      destruct (P <? Component.export C'I) eqn:Hproc_export.
-                      ***** (* valid call, the procedure is exported *)
-                            left.
-                            exists [ECall C P (Register.get Register.R_COM regs) C'].
-                            exists (C',(C,pc+1)::d,mem,regs,
-                                    EntryPoint.get C' P (genv_entrypoints G)).
-                            eapply Call; eauto.
-                            ****** unfold call_is_public_and_exists.
-                                   intros CI' Htarget_existence'.
-                                   rewrite Htarget_existence in Htarget_existence'.
-                                   inversion Htarget_existence' as [HC'IC'I'].
-                                   rewrite <- HC'IC'I'.
-                                   apply Nat.ltb_lt. auto.
-                            ****** unfold call_is_in_imports.
-                                   intros CI' Hcur_comp_existence'.
-                                   rewrite Hcur_comp_existence in Hcur_comp_existence'.
-                                   inversion Hcur_comp_existence' as [HCICI'].
-                                   rewrite <- HCICI'.
-                                   rewrite <- HC''C'. rewrite <- Hcomp_names. auto.
-                      ***** (* ERROR, the procedure is not exported *)
-                            right. right. left.
-                            unfold error_state.
-                            right. right. right. right. right. left.
-                            exists C'I, C', P. intros.
-                            unfold not. intro contra.
-                            apply Nat.ltb_lt in contra.
-                            rewrite Hproc_export in contra. inversion contra.
-                 **** (* the target has not been imported *)
-                      right. right. left.
-                      unfold error_state.
-                      right. right. right. right. left.
-                      exists CI. exists C'. exists P. intros.
-                      unfold not. intro contra.
-                      pose (find_none
-                              (fun entry : nat * nat =>
-                                 let (C'', P') := entry in (C'' =? C') && (P' =? P))
-                              (Component.import CI)
-                              Hcomponent_import (C',P) contra) as contra'.
-                      simpl in contra'. unfold andb in contra'.
-                      rewrite <- beq_nat_refl, <- beq_nat_refl in contra'.
-                      inversion contra'.
-             *** (* ERROR, call to a component that doesn't exist *)
-                 unfold error_state.
-                 right. right. left.
-                 right. right. right. left.
-                 exists C', P. intros. auto.
-          ** (* ERROR, we cannot check priviledges for the call *)
-             right. right. left.
-             unfold error_state.
-             right. right. left.
-             exists C, P. intros. auto.
-      (* RETURN *)
-      + (* case analysis on the stack *)
-        destruct d as [? | [C' addr] d'] eqn:Hstack.
-        (* ERROR, empty stack *)
-        * unfold error_state. auto 11.
-        (* non-empty stack, check the target component *)
-        * destruct (C' =? C) eqn:Hreturn_target.
-          (* ERROR, return to same component *)
-          ** unfold error_state.
-             rewrite beq_nat_true_iff in Hreturn_target.
-             rewrite Hreturn_target.
-             eauto 13.
-          (* valid return *)
-          ** left.
-             exists [ERet C (Register.get Register.R_COM regs) C'].
-             exists (C',d',mem,regs,addr).
-             rewrite beq_nat_false_iff in Hreturn_target.
-             eapply Return; eauto.
-      (* HALT *)
-      + unfold final_state. auto.
-    (* we can't step because of a decode error *) 
-    - unfold error_state. auto.
-  Qed.
-      
   Theorem determinism:
     forall G s t s1 s2,
-      G |-CS s =>[t] s1 ->
-      G |-CS s =>[t] s2 ->
-      s1 = s2.
+      step G s t s1 -> step G s t s2 -> s1 = s2.
   Proof.
-    intros G s t s1 s2 E1 E2.
-    inversion E1; subst; inversion E2; subst;
-      (* trivial cases *)
-      try reflexivity;
-      (* contradiction: different instructions at the same address *)
-      try (match goal with
-           | Hexec : executing _ ?COMP ?MEM ?PC,
-             Hexec' : executing _ ?COMP ?MEM ?PC |- _ =>
-             unfold executing in Hexec, Hexec';
-             rewrite Hexec in Hexec';
-             inversion Hexec'; subst; auto
-           end);
-      (* contradiction: different values in the same register *)
-      try (match goal with
-           | Hreg_neq : Register.get _ _ <> 0,
-             Hreg_eq : Register.get _ _ = 0 |- _ =>
-             exfalso; apply Hreg_neq; apply Hreg_eq
-           end).
-    (* load from the same memory address *)
-    - match goal with
-      | Hmemget1 : Some _ = Memory.get mem _ _,
-        Hmemget2 : Some _ = Memory.get mem _ _ |- _ =>
-        rewrite <- Hmemget1 in Hmemget2;
-        inversion Hmemget2; subst; auto
-      end.
-    (* store at the same memory address *)
-    - match goal with
-      | Hmemset1 : Some _ = Memory.set mem C _ _,
-        Hmemset2 : Some _ = Memory.set mem C _ _ |- _ =>
-        rewrite <- Hmemset1 in Hmemset2;
-        inversion Hmemset2; subst; auto
-      end.
-    (* return exactly to same component and address *)
-    - match goal with
-      | Hstack : (C', pc') :: d' = (_, _) :: _ |- _ =>
-        inversion Hstack; subst; auto
-      end.
-  Qed.
-
-  (* auxiliary lemmas *)
-
-  Lemma step_implies_memory_existence:
-    forall G s t s',
-      G |-CS s =>[t] s' ->
-      exists Cmem, M.MapsTo (comp_of_state s) Cmem (mem_of_state s).
-  Proof.
-    intros G s t s'.
-    intros Hstep.
-    destruct s
-      as [[[[C d] mem] regs] pc] eqn:Hstate_s.
-    inversion Hstep; subst;
-      match goal with
-      | Hexec : executing ?INSTR C mem ?PC |- _ =>
-        unfold executing, Memory.get in Hexec;
-          destruct (M.find (elt:=list nat) C mem)
-          as [Cmem | ] eqn:HCmem;
-          [ exists Cmem; simpl;
-            apply (M.find_2 HCmem)
-          | rewrite EncDec.decode_nothing in Hexec;
-            inversion Hexec ]
-      end.
-  Qed.
-
-  Lemma MapsTo_extraction:
-    forall C cmem val (mem : M.t (list nat)),
-      M.MapsTo C cmem (M.add C val mem) ->
-      cmem = val.
-  Proof.
-    intros.
-    apply F.add_mapsto_iff in H.
-    destruct H.
-    - destruct H. symmetry. auto.
-    - exfalso. destruct H. destruct H. auto.
-  Qed.
-
-  Lemma epsilon_step_weakening:
-    forall Is E C d1 mem mem' cmem cmem' regs regs' pc pc',
-      let G := mkGlobalEnv Is E in
-      M.MapsTo C cmem  mem ->
-      M.MapsTo C cmem' mem' ->
-      G |-CS (C,d1,mem,regs,pc) =>[E0] (C,d1,mem',regs',pc') ->
-      forall E' d2 wmem,
-        let G' := mkGlobalEnv Is E' in
-        M.MapsTo C cmem wmem ->
-        (G' |-CS (C,d2,wmem,regs,pc) =>[E0] (C,d2,wmem,regs',pc'))
-        \/
-        (forall wmem',
-         wmem' = M.add C cmem' wmem ->
-         G' |-CS (C,d2,wmem,regs,pc) =>[E0] (C,d2,wmem',regs',pc')).
-  Proof.
-    intros Is E C d1 mem mem' cmem cmem' regs regs' pc pc'.
-    intros G HCmem HCmem' Hstep.
-    intros E' d2 wmem G' HCwmem.
-    inversion Hstep; subst.
-    - left. apply Nop; auto.
-    - left. apply Const with r cval; auto.
-    - left. apply Mov with r1 r2; auto.
-    - left. eapply BinOp; eauto.
-    - left. eapply Load; try reflexivity.
-      + assert (Hexec':
-          executing (IntermediateMachine.Load r1 r2) C wmem pc). {
-          unfold executing. unfold executing in H5.
-          unfold Memory.get. unfold Memory.get in H5.
-          rewrite (M.find_1 HCwmem).
-          rewrite (M.find_1 HCmem') in H5.
-          apply H5.
-        } apply Hexec'.
-      + assert (cmem = cmem'). {
-          apply (F.MapsTo_fun HCmem HCmem').
-        }
-        unfold Memory.get. unfold Memory.get in H9.
-        rewrite (M.find_1 HCwmem), H.
-        rewrite (M.find_1 HCmem') in H9.
-        apply H9.
-    - unfold Memory.set in H10. 
-      rewrite (M.find_1 HCmem) in H10. inversion H10. subst.
-      remember (Register.get r1 regs') as r1val.
-      remember (Register.get r2 regs') as r2val.
-      right. intros wmem' HCwmem'.
-      apply Store with r1 r2 r1val r2val; auto.
-      unfold Memory.set in HCmem'.
-      apply MapsTo_extraction in HCmem'.
-      unfold Memory.set.
-      rewrite (M.find_1 HCwmem).
-      rewrite HCmem' in HCwmem'.
-      rewrite HCwmem'. auto.
-    - left. eapply Jal; eauto.
-    - left. eapply Jump; eauto.
-    - left. eapply BnzNZ.
-      + assert (executing
-                  (IntermediateMachine.Bnz r offset) C wmem pc). {
-          unfold executing. unfold executing in H1.
-          unfold Memory.get. unfold Memory.get in H1.
-          rewrite (M.find_1 HCwmem).
-          rewrite (M.find_1 HCmem') in H1.
-          apply H1.
-        } eauto.
-      + auto.
-    - left. eapply BnzZ.
-      + assert (executing
-                  (IntermediateMachine.Bnz r offset) C wmem pc). {
-          unfold executing. unfold executing in H1.
-          unfold Memory.get. unfold Memory.get in H1.
-          rewrite (M.find_1 HCwmem).
-          rewrite (M.find_1 HCmem') in H1.
-          apply H1.
-        } eauto.
-      + auto.
-  Qed.
+  Admitted.
 End CS.
