Intermediate/Machine.v
@@ -1,27 +1,51 @@
 Require Import Common.Definitions.
 Require Import Common.Util.
+Require Export Common.Values.
+Require Export Common.Linking.
 
-Require Import Coq.FSets.FMapAVL.
-Require Import Coq.FSets.FMapFacts.
-Require Import Coq.Structures.OrdersEx.
-Require Import Coq.Structures.OrdersAlt.
+Module Intermediate.
 
-Module IntermediateMachine.
+Inductive register : Type :=
+  R_ONE | R_COM | R_AUX1 | R_AUX2 | R_RA | R_SP.
 
-Module backNat_as_OT := Backport_OT Nat_as_OT.
-Module M := FMapAVL.Make backNat_as_OT.
-Module P := WProperties_fun Nat_as_OT M.
-Module F := P.F.
+Definition label := nat.
+
+Inductive imvalue : Type :=
+| IInt : nat -> imvalue
+| IPtr : Pointer.t -> imvalue.
+
+Definition imm_to_val (im : imvalue) : value :=
+  match im with
+  | IInt n => Int n
+  | IPtr p => Ptr p
+  end.
+
+Inductive instr :=
+| Nop : instr
+| Label : label -> instr
+(* register operations *)
+| Const : imvalue -> register -> instr
+| Mov : register -> register -> instr
+| BinOp : binop -> register -> register -> register -> instr
+(* memory operations *)
+| Load : register -> register -> instr
+| Store : register -> register -> instr
+| Alloc : register -> register -> instr
+(* conditional and unconditional jumps *)
+| Bnz : register -> label -> instr
+| Jump : register -> instr
+| Jal : label -> instr
+(* components interaction *)
+| Call : Component.id -> Procedure.id -> instr
+| Return : instr
+(* termination *)
+| Halt : instr.
 
 Module Register.
-  Definition data : Type := M.t nat.
+  Definition t : Type := list value.
 
-  Inductive reg : Set :=
-    R_PC | R_ONE | R_COM | R_AUX1 | R_AUX2 | R_RA | R_SP.
-
-  Definition to_nat (r : reg) : nat :=
+  Definition to_nat (r : register) : nat :=
     match r with
-    | R_PC   => 0
     | R_ONE  => 1
     | R_COM  => 2
     | R_AUX1 => 3
@@ -30,167 +54,80 @@ Module Register.
     | R_SP   => 6
     end.
 
-  Definition empty :=
-    M.add (to_nat R_PC)   0 (
-    M.add (to_nat R_ONE)  0 (
-    M.add (to_nat R_COM)  0 (
-    M.add (to_nat R_AUX1) 0 (
-    M.add (to_nat R_AUX2) 0 (
-    M.add (to_nat R_RA)   0 (
-    M.add (to_nat R_SP)   0 (
-    M.empty nat))))))).
+  Definition init := repeat Undef 7.
 
-  Definition get (r : reg) (regs : data) : nat :=
-    match M.find (to_nat r) regs with
+  Definition get (r : register) (regs : t) : value :=
+    match nth_error regs (to_nat r) with
     | Some val => val
     (* this should never happen (i.e. regs should be well-formed) *)
-    | None => 0
+    | None => Undef
     end.
 
-  Definition set (r : reg) (val : nat) (regs : data) : data :=
-    M.add (to_nat r) val regs.
+  Definition set (r : register) (val : value) (regs : t) : t :=
+    Util.Lists.update regs (to_nat r) val.
 
-  Lemma empty_memory_wf:
-    forall r, exists val, M.MapsTo (to_nat r) val empty.
+  Definition invalidate (regs : t) : t :=
+    [Undef; Undef; get R_COM regs; Undef; Undef; get R_RA regs; Undef].
+
+  Lemma init_registers_wf:
+    forall r, exists val, get r init = val.
   Proof.
-    intro r.
-    eexists. unfold empty.
-    induction r;
-      [
-      | apply M.add_2; simpl; auto
-      | apply M.add_2; simpl; auto;
-        apply M.add_2; auto
-      | apply M.add_2; simpl; auto;
-        apply M.add_2; simpl; auto;
-        apply M.add_2; auto
-      | apply M.add_2; simpl; auto;
-        apply M.add_2; simpl; auto;
-        apply M.add_2; simpl; auto;
-        apply M.add_2; auto
-      | apply M.add_2; simpl; auto;
-        apply M.add_2; simpl; auto;
-        apply M.add_2; simpl; auto;
-        apply M.add_2; simpl; auto;
-        apply M.add_2; auto
-      | apply M.add_2; simpl; auto;
-        apply M.add_2; simpl; auto;
-        apply M.add_2; simpl; auto;
-        apply M.add_2; simpl; auto;
-        apply M.add_2; simpl; auto;
-        apply M.add_2; auto ];
-      apply M.add_1; auto.
+    intros r. unfold get.
+    exists Undef. destruct r; auto.
   Qed.
 End Register.
 
-Module Memory.
-  Definition address := nat.
-  Definition data: Type := M.t (list nat).
-
-  Definition get mem C a : option nat :=
-    match M.find C mem with
-    (* when the address 'a' points outside of memory, we just return 0 *)
-    | Some cmem => Some (nth a cmem 0)
-    | None => None
-    end.
-
-  Fixpoint local_update (a : address) (val : nat) (lmem : list nat) :=
-    match lmem with
-    | [] =>
-      (* extend the memory, since the address points outside of it *)
-      (* (we are modeling an infinite memory, hence this extension) *)
-      match a with
-      | 0 => [val]
-      | S a' => 0 :: local_update a' val []
-      end
-    | val' :: lmem' =>
-      match a with
-      | 0 => val :: lmem'
-      | S a' => val' :: local_update a' val lmem'
-      end
-    end.
-
-  Definition set mem C a val :=
-    match M.find C mem with
-    | Some cmem => Some (M.add C (local_update a val cmem) mem)
-    | None => None
-    end.
-End Memory.
- 
-Inductive binop := Add | Minus | Mul | Eq | Leq.
-
-Inductive instr :=
-| Nop    : instr
-(* register operations *)
-| Const  : nat -> Register.reg -> instr
-| Mov    : Register.reg -> Register.reg -> instr
-| BinOp  : binop -> Register.reg -> Register.reg -> Register.reg -> instr
-(* memory operations *)
-| Load   : Register.reg -> Register.reg -> instr
-| Store  : Register.reg -> Register.reg -> instr
-(* conditional and unconditional jumps *)
-| Bnz    : Register.reg -> nat -> instr
-| Jump   : Register.reg -> instr
-| Jal    : Register.reg -> instr
-(* components interaction *)
-| Call   : Component.id -> Procedure.id -> instr
-| Return : instr
-(* termination *)
-| Halt   : instr.
-
-Module EncDec.
-  (* we assume to have a decoder for our instructions. Later we could try
-     to think of a simple representation for instructions and implement
-     it for real *)
-
-  Definition decode (n : option nat) : option instr := admit.
-  Definition encode (i:instr) : option nat := admit.
-
-  Theorem decode_encode : forall i, decode (encode i) = Some i.
-  Proof. Admitted.
-  Theorem decode_nothing : decode None = None. Proof. Admitted.
-End EncDec.
-
 Module EntryPoint.
-  Definition data : Type := M.t (list Memory.address).
+  Definition t := NMap.t (NMap.t Block.id).
 
-  Definition get C P E : Memory.address :=
-    match M.find C E with
-    | Some E' => nth P E' 0
-    | None => 0
+  Definition get C P E : option Block.id :=
+    match NMap.find C E with
+    | Some addrs => NMap.find P addrs
+    | None => None
     end.
 
   Lemma get_on_compatible_entrypoints :
     forall E E' C P addrs,
-      M.MapsTo C addrs E ->
-      M.MapsTo C addrs E' ->
+      NMap.MapsTo C addrs E ->
+      NMap.MapsTo C addrs E' ->
       get C P E = get C P E'.
   Proof.
     intros E E' C P addrs HEaddrs HE'addrs.
     unfold get.
-    rewrite F.find_mapsto_iff in HEaddrs, HE'addrs.
+    rewrite NMapFacts.find_mapsto_iff in HEaddrs, HE'addrs.
     rewrite <- HEaddrs in HE'addrs.
     inversion HE'addrs as [HEeqE'].
     rewrite HEeqE'.
     reflexivity.
   Qed.
+
+  Definition mergeable (e1 e2 : t) : Prop := NMapExtra.Disjoint e1 e2.
+  
+  Definition merge (e1 e2 : t) (mergeable_prf : mergeable e1 e2) : t :=
+    NMapExtra.update e1 e2.
 End EntryPoint.
 
-(* auxiliary definitions *)
+(* programs *)
 
-Definition call_is_public_and_exists
-           (Is : Program.interface)
-           (C : Component.id) (P : Procedure.id) :=
-  forall CI,
-    find (fun C' => C =? Component.name C') Is = Some CI ->
-    P < Component.export CI.
+Definition code := list instr.
 
-Definition call_is_in_imports
-           (Is : Program.interface)
-           (C C': Component.id) (P : Procedure.id) :=
-  forall CI,
-    find (fun C' => C =? Component.name C') Is = Some CI ->
-    In (C',P) (Component.import CI).
+Record program := {
+  prog_interface : Program.interface;
+  prog_procedures : NMap.t (NMap.t code);
+  prog_buffers : NMap.t (list (Block.id * nat));
 
-Definition executing i C mem pc :=
-  EncDec.decode (Memory.get mem C pc) = Some i.
-End IntermediateMachine.
+  (* interface soundness *)
+  prog_interface_soundness:
+    sound_interface prog_interface;
+
+  (* procedure soundness: TODO *)
+
+  (* buffers soundness w.r.t. the interface *)
+  prog_buffers_soundness:
+    forall C, NMap.In C prog_buffers <-> NMap.In C prog_interface
+}.
+
+Definition closed_program (p : program) :=
+  closed_interface (prog_interface p).
+
+End Intermediate.
