Intermediate/PS.v
@@ -2,355 +2,163 @@ Require Import Common.Definitions.
 Require Import Common.Util.
 Require Import Common.Events.
 Require Import Common.Smallstep.
+Require Import Common.Memory.
 Require Import Intermediate.Machine.
+Require Import Intermediate.GlobalEnv.
 Require Import Intermediate.CS.
 
 Module PS.
-  Import IntermediateMachine.
+  Import Intermediate.
 
-  Record program := {
-    prog_interface : Program.interface;
-    prog_memory : Memory.data;
-    prog_entrypoints : EntryPoint.data;
-    prog_split : list Component.id;
-    prog_entrypoints_wf :
-      forall CI C,
-        In CI prog_interface ->
-        Component.name CI = C ->
-        In C prog_split ->
-        M.In C prog_entrypoints /\
-        exists addrs, M.MapsTo C addrs prog_entrypoints;
-    prog_split_wf :
-      forall C,
-        In C prog_split ->
-        exists CI, In CI prog_interface /\ Component.name CI = C
-  }.
+  Module PartialPointer.
+    Definition t : Type := Component.id * option (Block.id * Block.offset).
+  End PartialPointer.
 
-  Definition stack := list (Component.id * option Memory.address).
+  Definition stack := list PartialPointer.t.
 
-  Definition program_state : Type :=
-    Component.id * stack * Memory.data * Register.data * Memory.address.
-  Definition context_state : Type :=
-    Component.id * stack * Memory.data.
+  Definition program_state : Type := stack * Memory.t * Register.t * Pointer.t.
+  Definition context_state : Type := stack * Memory.t * Component.id.
 
-  Inductive exec_state : Type :=
-  | Normal
-  | WentWrong.
+  Inductive state : Type :=
+  | PC : program_state -> state
+  | CC : context_state -> state.
 
-  Inductive partial_state : Type :=
-  | PC : program_state -> partial_state
-  | CC : context_state -> exec_state -> partial_state.
-
-  Definition to_partial_frame pc frame : Component.id * option Memory.address :=
-    match frame with (C,i) =>
-      if Util.mem C pc then (C, Some i) else (C, None)
-    end.
+  Definition to_partial_frame pc frame : PartialPointer.t :=
+    let '(C, b, o) := frame in
+    if Util.Lists.mem C pc then
+      (C, Some (b, o))
+    else
+      (C, None).
 
   Definition to_partial_stack (s : CS.stack) (pc : list Component.id) :=
     map (to_partial_frame pc) s.
 
   Lemma push_by_prog_preserves_partial_stack :
-    forall s ps pc C i,
-      Util.mem C pc = true ->
+    forall s ps pc C b o,
+      Util.Lists.mem C pc = true ->
       to_partial_stack s pc = ps ->
-      to_partial_stack ((C,i)::s) pc = (C,Some i) :: ps.
+      to_partial_stack ((C,b,o)::s) pc = (C,Some (b,o)) :: ps.
   Proof.
-    intros s ps pc C i Hprogturn H.
+    intros s ps pc C b o Hprogturn H.
     simpl. rewrite Hprogturn. rewrite H. reflexivity.
   Qed.
 
   Lemma push_by_context_preserves_partial_stack :
-    forall s ps pc C i,
+    forall s ps pc C b o,
       ~ (In C pc) ->
       to_partial_stack s pc = ps ->
-      to_partial_stack ((C,i)::s) pc = (C,None) :: ps.
+      to_partial_stack ((C,b,o)::s) pc = (C,None) :: ps.
   Proof.
-    intros s ps pc C i Hprogturn Hpstack.
-    simpl. apply Util.not_in_iff_mem_false in Hprogturn.
+    intros s ps pc C b o Hprogturn Hpstack.
+    simpl. apply Util.Lists.not_in_iff_mem_false in Hprogturn.
     rewrite Hprogturn. rewrite Hpstack. reflexivity.
   Qed.
 
-  Record global_env := mkGlobalEnv {
-    genv_interfaces : Program.interface;
-    genv_entrypoints : EntryPoint.data;
-    genv_split : list Component.id;
-  }.
+  (* The split between program and context is represented by the domain of the
+     entrypoints map. *)
+  Definition is_program_component G C := NMap.In C (genv_entrypoints G).
+  Definition is_context_component G C := ~ is_program_component G C.
 
-  Definition initial_state_for
-             (p : program) (split : list Component.id) : partial_state :=
-    let mem := prog_memory p in
-    let E := prog_entrypoints p in
-    let split := prog_split p in
-    if Util.mem 0 split then
-      PC (0, [], mem, Register.empty, EntryPoint.get 0 0 E)
-    else
-      CC (0, [], mem) Normal.
-
-  Definition initial_state p (s : partial_state) : Prop :=
-    match s with
-    | PC (C, d, mem, regs, pc) =>
-      C = 0 /\ d = [] /\ regs = Register.empty /\
-      pc = EntryPoint.get 0 0 (prog_entrypoints p)
-    | CC (C, d, mem) state =>
-      C = 0 /\ d = []
-    end.
-
-  Definition final_state (s : partial_state) : Prop :=
-    match s with
-    | PC (C, d, mem, regs, pc) =>
-      executing Halt C mem pc
-    | CC (C, d, mem) state =>
-      state = Normal
-    end.
-
-  Definition is_program_component C (prog_comps : list Component.id) :=
-    In C prog_comps.
-  Definition is_context_component C (prog_comps : list Component.id) :=
-    ~ (In C prog_comps).
-
-  Definition maps_match_on {T : Type} split (map map' : M.t T) :=
-    forall C Cmap,
-      PS.is_program_component C split ->
-      (M.MapsTo C Cmap map <-> M.MapsTo C Cmap map').
-
-  Reserved Notation "G |-PS s1 '=>[' t ']' s2" (at level 40).
-
-  Inductive step (G : global_env)
-    : partial_state -> trace -> partial_state -> Prop :=
+  Inductive step (G : global_env) : state -> trace -> state -> Prop :=
   | Program_Epsilon:
-      forall E C s ps
-             mem mem' wmem wmem' cmem cmem'
-             regs regs' pc pc',
-        M.MapsTo C cmem wmem ->
-        M.MapsTo C cmem' wmem' ->
-        maps_match_on (genv_split G) E (genv_entrypoints G) ->
-        let G' := CS.mkGlobalEnv (genv_interfaces G) E in
-        CS.step G' (C,s,wmem,regs,pc) E0 (C,s,wmem',regs',pc') ->
-        M.MapsTo C cmem mem ->
-        M.MapsTo C cmem' mem' ->
-        G |-PS (PC (C,ps,mem,regs,pc)) =>[E0] (PC (C,ps,mem',regs',pc'))
+      forall gps pgps
+             (mem mem' wmem wmem' : Memory.t) cmem cmem'
+             (regs regs' : Register.t) (pc pc' : Pointer.t),
+        let C := Pointer.component pc in
+        NMap.MapsTo C cmem wmem ->
+        NMap.MapsTo C cmem' wmem' ->
+        CS.step G (gps,wmem,regs,pc) E0 (gps,wmem',regs',pc') ->
+        NMap.MapsTo C cmem mem ->
+        NMap.MapsTo C cmem' mem' ->
+        step G (PC (pgps,mem,regs,pc)) E0 (PC (pgps,mem',regs',pc'))
 
   | Program_Internal_Call:
-      forall mem C pc regs d d' C' P,
-        executing (Call C' P) C mem pc ->
+      forall pgps pgps' mem regs b o pc C' P val,
+        executing G pc (Call C' P) ->
+        let C := Pointer.component pc in
         C' <> C ->
-        call_is_public_and_exists (genv_interfaces G) C' P ->
-        call_is_in_imports (genv_interfaces G) C C' P ->
-        is_program_component C' (genv_split G) ->
-        d' = (C,Some (pc+1)) :: d ->
-        let t := [ECall C P (Register.get Register.R_COM regs) C'] in
-        G |-PS (PC (C,d,mem,regs,pc)) =>[t]
-                (PC (C',d',mem,regs,EntryPoint.get C' P (genv_entrypoints G)))
+        imported_procedure (genv_interface G) C C' P ->
+        is_program_component G C' ->
+        pgps' = (C, Some (b, o)) :: pgps ->
+        EntryPoint.get C' P (genv_entrypoints G) = Some b ->
+        Register.get R_COM regs = Int val ->
+        let pc' := (C', b, 0) in
+        let t := [ECall C P val C'] in
+        step G (PC (pgps,mem,regs,pc)) t (PC (pgps',mem,regs,pc'))
 
   | Program_Internal_Return:
-      forall mem C C' pc pc' d d' regs,
-        executing Return C mem pc ->
+      forall pgps pgps' mem regs pc pc' C' b o val,
+        let C := Pointer.component pc in
+        executing G pc Return ->
+        pgps = (C', Some (b,o)) :: pgps' ->
         C' <> C ->
-        is_program_component C' (genv_split G) ->
-        d = (C',Some pc') :: d' ->
-        let t := [ERet C (Register.get Register.R_COM regs) C'] in
-        G |-PS (PC (C,d,mem,regs,pc)) =>[t] (PC (C',d',mem,regs,pc'))
+        is_program_component G C' ->
+        Register.get R_COM regs = Int val ->
+        let t := [ERet C val C'] in
+        step G (PC (pgps,mem,regs,pc)) t (PC (pgps',mem,regs,pc'))
 
   | Program_External_Call:
-      forall mem C pc regs d d' C' P,
-        executing (Call C' P) C mem pc ->
+      forall pgps pgps' mem regs pc C' b o P val,
+        let C := Pointer.component pc in
+        executing G pc (Call C' P) ->
         C' <> C ->
-        call_is_public_and_exists (genv_interfaces G) C' P ->
-        call_is_in_imports (genv_interfaces G) C C' P ->
-        is_context_component C' (genv_split G) ->
-        d' = (C,Some (pc+1)) :: d ->
-        let t := [ECall C P (Register.get Register.R_COM regs) C'] in
-        G |-PS (PC (C,d,mem,regs,pc)) =>[t] (CC (C',d',mem) Normal)
+        imported_procedure (genv_interface G) C C' P ->
+        is_context_component G C' ->
+        pgps' = (C, Some (b,o)) :: pgps ->
+        Register.get R_COM regs = Int val ->
+        let t := [ECall C P val C'] in
+        step G (PC (pgps,mem,regs,pc)) t (CC (pgps',mem,C'))
 
   | Program_External_Return:
-      forall mem C C' pc d d' regs,
-        executing Return C mem pc ->
+      forall pgps pgps' mem regs pc C' val,
+        let C := Pointer.component pc in
+        executing G pc Return ->
         C' <> C ->
-        is_context_component C' (genv_split G) ->
-        d = (C',None) :: d' ->
-        let t := [ERet C (Register.get Register.R_COM regs) C'] in
-        G |-PS (PC (C,d,mem,regs,pc)) =>[t] (CC (C',d',mem) Normal)
+        is_context_component G C' ->
+        pgps = (C', None) :: pgps' ->
+        Register.get R_COM regs = Int val ->
+        let t := [ERet C val C'] in
+        step G (PC (pgps,mem,regs,pc)) t (CC (pgps',mem,C'))
 
   | Context_Epsilon:
-      forall mem C d,
-        G |-PS (CC (C,d,mem) Normal) =>[E0] (CC (C,d,mem) Normal)
-
-  | Context_GoesWrong:
-      forall mem C d,
-        G |-PS (CC (C,d,mem) Normal) =>[E0] (CC (C,d,mem) WentWrong)
+      forall pgps mem C,
+        step G (CC (pgps,mem,C)) E0 (CC (pgps,mem,C))
 
   | Context_Internal_Call:
-      forall mem C d d' C' P call_arg,
+      forall pgps pgps' mem C C' P call_arg,
         C' <> C ->
-        call_is_public_and_exists (genv_interfaces G) C' P ->
-        call_is_in_imports (genv_interfaces G) C C' P ->
-        is_context_component C' (genv_split G) ->
-        d' = (C,None) :: d ->
+        imported_procedure (genv_interface G) C C' P ->
+        is_context_component G C' ->
+        pgps' = (C, None) :: pgps ->
         let t := [ECall C P call_arg C'] in
-        G |-PS (CC (C,d,mem) Normal) =>[t] (CC (C',d',mem) Normal)
+        step G (CC (pgps,mem,C)) t (CC (pgps',mem,C'))
 
   | Context_Internal_Return:
-      forall mem C C' d d' return_val,
+      forall pgps pgps' mem C C' return_val,
         C' <> C ->
-        is_context_component C' (genv_split G) ->
-        d = (C',None) :: d' ->
+        is_context_component G C' ->
+        pgps = (C', None) :: pgps' ->
         let t := [ERet C return_val C'] in
-        G |-PS (CC (C,d,mem) Normal) =>[t] (CC (C',d',mem) Normal)
+        step G (CC (pgps,mem,C)) t (CC (pgps',mem,C'))
 
   | Context_External_Call:
-      forall mem C regs d d' C' P,
+      forall pgps pgps' mem regs C C' P b val,
         C' <> C ->
-        call_is_public_and_exists (genv_interfaces G) C' P ->
-        call_is_in_imports (genv_interfaces G) C C' P ->
-        is_program_component C' (genv_split G) ->
-        d' = (C,None) :: d ->
-        let t := [ECall C P (Register.get Register.R_COM regs) C'] in
-        G |-PS (CC (C,d,mem) Normal) =>[t]
-                (PC (C',d',mem,regs,EntryPoint.get C' P (genv_entrypoints G)))
+        exported_procedure (genv_interface G) C' P ->
+        imported_procedure (genv_interface G) C C' P ->
+        is_program_component G C' ->
+        pgps' = (C, None) :: pgps ->
+        EntryPoint.get C' P (genv_entrypoints G) = Some b ->
+        Register.get R_COM regs = Int val ->
+        let t := [ECall C P val C'] in
+        let pc' := (C', b, 0) in
+        step G (CC (pgps,mem,C)) t (PC (pgps',mem,regs,pc'))
 
   | Context_External_Return:
-      forall mem C C' pc' d d' regs,
-        d = (C',Some pc') :: d' ->
-        is_program_component C' (genv_split G) ->
-        let t := [ERet C (Register.get Register.R_COM regs) C'] in
-        G |-PS (CC (C,d,mem) Normal) =>[t] (PC (C',d',mem,regs,pc'))
-
-  where "G |-PS s1 '=>[' t ']' s2" := (step G s1 t s2).
-
-  Lemma maps_match_on_reflexive :
-    forall T split (map : M.t T),
-      maps_match_on split map map.
-  Proof.
-    split; intros; auto.
-  Qed.
-
-  Lemma maps_match_on_symmetric :
-    forall T split (map1 map2 : M.t T),
-      maps_match_on split map1 map2 ->
-      maps_match_on split map2 map1.
-  Proof.
-    intros ? split map1 map2 Hmaps_match.
-    split; intro; apply Hmaps_match; auto.
-  Qed.
-
-  Hint Resolve maps_match_on_reflexive.
-  Hint Resolve maps_match_on_symmetric.
-
-  Lemma update_related_memories_generic :
-    forall split mem1 mem1' mem2 mem2' C Cmem C' addr val,
-      maps_match_on split mem1 mem2 ->
-      is_program_component C split ->
-      Some mem1' = Memory.set mem1 C' addr val ->
-      Some mem2' = Memory.set mem2 C' addr val ->
-      M.MapsTo C Cmem mem1' ->
-      M.MapsTo C Cmem mem2'.
-  Proof.
-    intros split mem1 mem1' mem2 mem2' C Cmem C' addr val.
-    intros Hmems_match HCorigin Hmem1upd Hmem2upd HCmem.
-    unfold Memory.set.
-    unfold Memory.set in HCmem.
-    destruct (C =? C') eqn:HeqCC'.
-    + apply beq_nat_true in HeqCC'. subst.
-      unfold Memory.set in Hmem1upd, Hmem2upd.
-      destruct (M.find (elt:=list nat) C' mem1) eqn:Hfind_mem1.
-      * destruct (M.find (elt:=list nat) C' mem2) eqn:Hfind_mem2.
-        ** inversion Hmem1upd as [Hmem1]. inversion Hmem2upd as [Hmem2].
-           subst. rewrite (CS.MapsTo_extraction _ _ _ _ HCmem).
-           enough (l = l0). subst.
-           apply M.add_1; auto.
-           apply F.find_mapsto_iff in Hfind_mem1.
-           apply F.find_mapsto_iff in Hfind_mem2.
-           apply Hmems_match in Hfind_mem1.
-           apply (F.MapsTo_fun Hfind_mem1 Hfind_mem2); auto.
-           auto.
-        ** inversion Hmem2upd.
-      * inversion Hmem1upd.
-    + apply beq_nat_false in HeqCC'.
-      unfold Memory.set in Hmem1upd, Hmem2upd.
-      destruct (M.find (elt:=list nat) C' mem1) eqn:Hfind_mem1.
-      * destruct (M.find (elt:=list nat) C' mem2) eqn:Hfind_mem2.
-        ** inversion Hmem1upd as [Hmem1]. inversion Hmem2upd as [Hmem2].
-           subst. apply M.add_2.
-           *** unfold not. intro. apply HeqCC'. symmetry. apply H.
-           *** apply Hmems_match.
-               **** assumption.
-               **** destruct (M.find (elt:=list nat) C' mem1) eqn:Hfind'.
-                    ***** eapply M.add_3.
-                    ****** intro. apply HeqCC'. symmetry. apply H.
-                    ****** apply HCmem.
-                    ***** inversion Hfind_mem1.
-        ** inversion Hmem2upd.
-      * inversion Hmem1upd.
-  Qed.
-
-  Lemma update_related_memories :
-    forall split mem1 mem1' mem2 mem2' C addr val,
-      maps_match_on split mem1 mem2 ->
-      Some mem1' = Memory.set mem1 C addr val ->
-      Some mem2' = Memory.set mem2 C addr val ->
-      maps_match_on split mem1' mem2'.
-  Proof.
-    intros split mem1 mem1' mem2 mem2' C addr val.
-    intros Hmems_match Hmem1'_ Hmem2'_.
-    unfold PS.maps_match_on.
-    intros C0 C0mem HC0_origin.
-    destruct (C =? C0) eqn:HCC0.
-    - rewrite beq_nat_true_iff in HCC0. subst. auto.
-      split.
-      apply update_related_memories_generic with
-          (mem1:=mem1) (mem2:=mem2) (C':=C0)
-          (split:=split) (addr:=addr) (val:=val);
-        auto.
-      apply update_related_memories_generic with
-          (mem1:=mem2) (mem2:=mem1) (C':=C0)
-          (split:=split) (addr:=addr) (val:=val);
-        auto.
-    - split.
-      apply update_related_memories_generic with
-          (mem1:=mem1) (mem2:=mem2) (C':=C)
-          (split:=split) (addr:=addr) (val:=val);
-        auto.
-      apply update_related_memories_generic with
-          (mem1:=mem2) (mem2:=mem1) (C':=C)
-          (split:=split) (addr:=addr) (val:=val);
-        auto.
-  Qed.  
-
-  Section SEMANTICS.
-    Variable p : program.
-
-    Definition semantics :=
-      @Semantics_gen partial_state global_env
-                     step
-                     (initial_state p)
-                     final_state
-                     (mkGlobalEnv (prog_interface p)
-                                  (prog_entrypoints p)
-                                  (prog_split p)).
-  End SEMANTICS.
-
-  (* if entrypoints are well-formed, then they remain
-     well-formed even if we consider only the ones relative
-     to the components in the split *)
-  Lemma entrypoints_exist_wrt_split split :
-    forall p CI C,
-      In CI (CS.prog_interface p) ->
-      Component.name CI = C ->
-      In C split ->
-      M.In C (CS.prog_entrypoints p) /\
-      exists addrs, M.MapsTo C addrs (CS.prog_entrypoints p).
-  Proof.
-    intros p CI C.
-    intros HCI_in_I HCI_name_is_C HC_in_split.
-    apply (CS.prog_entrypoints_wf p) with CI; assumption.
-  Qed.
-
-  Definition apply_split (p : CS.program) split splitWF :=
-    {| prog_interface := CS.prog_interface p;
-       prog_memory := CS.prog_memory p;
-       prog_entrypoints := CS.prog_entrypoints p;
-       prog_split := split;
-       prog_entrypoints_wf :=
-         entrypoints_exist_wrt_split split p;
-       prog_split_wf := splitWF |}.
+      forall pgps pgps' mem regs C C' b o val,
+        pgps = (C', Some (b,o)) :: pgps' ->
+        is_program_component G C' ->
+        Register.get R_COM regs = Int val ->
+        let t := [ERet C val C'] in
+        step G (CC (pgps,mem,C)) t (PC (pgps',mem,regs, (C',b,o))).
 End PS.
