Common/Linking.v
@@ -1,0 +1,29 @@
+Require Import Common.Definitions.
+Require Import Common.Util.
+
+(* an imported procedure is either open (the interface is missing)
+   or exported by the right component *)
+Definition sound_interface (interface : Program.interface) : Prop :=
+  forall C CI,
+    Program.has_component interface C CI ->
+  forall C' P,
+    Component.is_importing CI C' P ->
+  forall CI',
+    Program.has_component interface C' CI' ->
+    Component.is_exporting CI' P.
+
+(* an imported procedure is always exported by the right component *)
+Definition closed_interface (interface : Program.interface) : Prop :=
+  forall C CI,
+    Program.has_component interface C CI ->
+  forall C' P,
+    Component.is_importing CI C' P ->
+  exists CI',
+    Program.has_component interface C' CI' /\
+    Component.is_exporting CI' P.
+
+Definition mergeable_interfaces (i1 i2 : Program.interface) : Prop :=
+  NMapExtra.Disjoint i1 i2.
+
+Definition interface_merge (i1 i2 : Program.interface) (prf: mergeable_interfaces i1 i2) :=
+  NMapExtra.update i1 i2.
