Common/Maps.v
@@ -1,0 +1,9 @@
+Require Import Coq.FSets.FMapAVL.
+Require Import Coq.FSets.FMapFacts.
+Require Import Coq.Structures.OrdersEx.
+Require Import Coq.Structures.OrdersAlt.
+
+Module backNat_as_OT := Backport_OT Nat_as_OT.
+Module NMap := FMapAVL.Make backNat_as_OT.
+Module NMapExtra := WProperties_fun Nat_as_OT NMap.
+Module NMapFacts := NMapExtra.F.
