Common/Memory.v
@@ -1,0 +1,131 @@
+Require Import Common.Definitions.
+Require Import Common.Values.
+
+Module Type AbstractComponentMemory.
+  Parameter t : Type.
+
+  Parameter alloc : t -> nat -> t * Block.id.
+  Parameter load : t -> Block.id -> Block.offset -> option value.
+  Parameter store : t -> Block.id -> Block.offset -> value -> option t.
+
+  Axiom load_after_alloc:
+    forall m m' n b,
+      alloc m n = (m',b) ->
+    forall b' i,
+      b' <> b -> load m' b' i = load m b' i.
+
+  Axiom load_after_store:
+    forall m m' b i v,
+      store m b i v = Some m' ->
+    forall b' i',
+      ((b' <> b \/ i' <> i) /\ load m' b' i' = load m b' i') \/
+      load m' b' i' = Some v.
+End AbstractComponentMemory.
+
+Module ComponentMemory : AbstractComponentMemory.
+  Definition block := list value.
+
+  Record mem := mkMem {
+    content : NMap.t block;
+    nextblock : Block.id;
+  }.
+  Definition t := mem.
+
+  Definition alloc m (size : nat) : mem * Block.id :=
+    let fresh_block := nextblock m in
+    let chunk := repeat Undef size in
+    ({| content := NMap.add fresh_block chunk (content m);
+        nextblock := 1 + nextblock m |},
+     fresh_block).
+
+  Definition load m b i : option value :=
+    match NMap.find b (content m) with
+    | Some chunk => nth_error chunk i
+    | None => None
+    end.
+
+  Fixpoint block_update data offset val : option block :=
+    match data with 
+    | [] => None (* store out of bounds *)
+    | val' :: rest =>
+      match offset with
+      | 0 => Some (val :: rest) 
+      | S offset' =>
+        match block_update rest offset' val with
+        | Some rest' => Some (val' :: rest')
+        | None       => None (* propagate store out of bounds *)
+        end
+      end
+    end.
+  
+  Definition store m b i v : option mem :=
+    match NMap.find b (content m) with
+    | Some chunk =>
+      match block_update chunk i v with
+      | Some chunk' =>
+        Some {| content := NMap.add b chunk' (content m);
+                nextblock := nextblock m |}
+      | _ => None
+      end
+    | None => None
+    end.
+
+  Lemma load_after_alloc:
+    forall (m m' : mem) (n : nat) b,
+      alloc m n = (m',b) ->
+    forall b' i,
+      b' <> b -> load m' b' i = load m b' i.
+  Proof.
+    intros m m' n b Halloc b' i Hb'.
+    unfold alloc in Halloc. inversion Halloc. subst.
+  Admitted.
+
+  Lemma load_after_store:
+    forall m m' b i v,
+      store m b i v = Some m' ->
+    forall b' i',
+      ((b' <> b \/ i' <> i) /\ load m' b' i' = load m b' i') \/
+      load m' b' i' = Some v.
+  Proof.
+    intros m m' b i v Hstore b' i'.
+    destruct (b =? b') eqn:Hbeqb'.
+    - destruct (i =? i') eqn:Hieqi'.
+      + right. admit.
+      + left. split.
+        * right. admit.
+        * admit.
+    - left. split.
+      + left. admit.
+      + admit.
+  Admitted.
+End ComponentMemory.
+
+Module Memory.
+  Definition t := NMap.t ComponentMemory.t.
+
+  Definition alloc (mem : t) (C : Component.id) (size : nat) : option (t * Pointer.t) :=
+    match NMap.find C mem with
+    | Some memC =>
+      let '(memC', b) := ComponentMemory.alloc memC size in
+      Some (NMap.add C memC' mem, (C, b, 0))
+    | None => None
+    end.
+
+  Definition load (mem : t) (ptr : Pointer.t) : option value :=
+    let '(C, b, o) := ptr in
+    match NMap.find C mem with
+    | Some memC => ComponentMemory.load memC b o
+    | None => None
+    end.
+
+  Definition store (mem :t) (ptr : Pointer.t) (v : value) : option t :=
+    let '(C, b, o) := ptr in
+    match NMap.find C mem with
+    | Some memC =>
+      match ComponentMemory.store memC b o v with
+      | Some memC' => Some (NMap.add C memC' mem)
+      | None => None
+      end
+    | None => None
+    end.
+End Memory.
