Common/Values.v
@@ -1,0 +1,82 @@
+Require Import Common.Definitions.
+Require Import Common.Util.
+
+Module Block.
+  Definition id := nat.
+  Definition offset := nat.
+End Block.
+
+Module Pointer.
+  Definition t : Type := Component.id * Block.id * Block.offset.
+
+  Definition component (p : t) : Component.id :=
+    let '(C, _, _) := p in C.
+
+  Definition block (p : t) : Block.id :=
+    let '(_, b, _) := p in b.
+
+  Definition offset (p : t) : Block.offset :=
+    let '(_, _, o) := p in o.
+
+  Definition eq (p1 p2 : t) : bool :=
+    let '(C1, b1, o1) := p1 in
+    let '(C2, b2, o2) := p2 in
+    (C1 =? C2) && (b1 =? b2) && (o1 =? o2).
+
+  Definition leq (p1 p2 : t) : option bool :=
+    let '(C1, b1, o1) := p1 in
+    let '(C2, b2, o2) := p2 in
+    if (C1 =? C2) && (b1 =? b2) then
+      Some (o1 <=? o2)
+    else
+      None.
+
+  Definition add (ptr : t) (offset : nat) : t :=
+    let '(C, b, o) := ptr in (C, b, o+offset).
+
+  Definition sub (ptr : t) (offset : nat) : option t :=
+    let '(C, b, o) := ptr in
+    match Util.Nat.safe_sub o offset with
+    | Some o' => Some (C, b, o')
+    | None => None
+    end.
+
+  Definition inc (ptr : t) : t := add ptr 1.
+End Pointer.
+
+Inductive value : Type :=
+| Int : nat -> value
+| Ptr : Pointer.t -> value
+| Undef : value.
+
+Inductive binop := Add | Minus | Mul | Eq | Leq.
+
+Definition eval_binop (op : binop) (v1 v2 : value) : value :=
+  match op, v1, v2 with
+  (* natural numbers *)
+  | Add,   Int n1, Int n2 => Int (n1 + n2)
+  | Minus, Int n1, Int n2 => Int (n1 - n2)
+  | Mul,   Int n1, Int n2 => Int (n1 * n2)
+  | Eq,    Int n1, Int n2 => Int (Util.Nat.of_bool (n1  =? n2))
+  | Leq,   Int n1, Int n2 => Int (Util.Nat.of_bool (n1 <=? n2))
+  (* pointer arithmetic *)
+  | Add,   Ptr p,  Int n  => Ptr (Pointer.add p n)
+  | Add,   Int n,  Ptr p  => Ptr (Pointer.add p n)
+  | Minus, Ptr p1, Ptr p2 => let '(C1, b1, o1) := p1 in
+                             let '(C2, b2, o2) := p2 in
+                             if (C1 =? C2) && (b1 =? b2) then
+                               Int (o1 - o2)
+                             else
+                               Undef
+  | Minus, Ptr p,  Int n  => match Pointer.sub p n with
+                             | Some p' => Ptr p'
+                             | None    => Undef
+                             end
+  | Eq,    Ptr p1, Ptr p2 => Int (Util.Nat.of_bool (Pointer.eq p1 p2))
+  | Leq,   Ptr p1, Ptr p2 => match Pointer.leq p1 p2 with
+                             | Some res => Int (Util.Nat.of_bool res)
+                             | None     => Undef
+                             end
+  (* undefined operations *)
+  | _,     _,       _       => Undef
+  end.
