Intermediate/GlobalEnv.v
@@ -1,0 +1,60 @@
+Require Import Common.Definitions.
+Require Import Intermediate.Machine.
+
+Import Intermediate.
+
+Record global_env := mkGlobalEnv {
+  genv_interface : Program.interface;
+  genv_procedures : NMap.t (NMap.t code);
+  genv_entrypoints : EntryPoint.t;
+}.
+
+Definition executing G (pc : Pointer.t) (i : instr) : Prop :=
+  exists C_procs P_code,
+    NMap.find (Pointer.component pc) (genv_procedures G) = Some C_procs /\
+    NMap.find (Pointer.block pc) C_procs = Some P_code /\
+    nth_error P_code (Pointer.offset pc) = Some i.
+
+Fixpoint find_label (c : code) (l : label) : option nat :=
+  let fix aux c o :=
+      match c with
+      | [] => None
+      | Label l' :: c' =>
+        if l =? l' then
+          Some o
+        else
+          aux c' (1+o)
+      | _ :: c' =>
+        aux c' (1+o)
+      end
+  in aux c 0.
+
+Definition find_label_in_procedure G (pc : Pointer.t) (l : label) : option Pointer.t :=
+  match NMap.find (Pointer.component pc) (genv_procedures G) with
+  | Some C_procs =>
+    match NMap.find (Pointer.block pc) C_procs with
+    | Some P_code =>
+      match find_label P_code l with
+      | Some offset => Some (Pointer.component pc, Pointer.block pc, offset)
+      | None => None
+      end
+    | None => None
+    end
+  | None => None
+  end.
+
+Definition find_label_in_component G (pc : Pointer.t) (l : label) : option Pointer.t :=
+  match NMap.find (Pointer.component pc) (genv_procedures G) with
+  | Some C_procs =>
+    let fix search ps :=
+        match ps with
+        | [] => None
+        | (p_block,p_code) :: ps' =>
+          match find_label_in_procedure G (Pointer.component pc, p_block, 0) l with
+          | None => search ps'
+          | Some ptr => Some ptr
+          end
+        end
+    in search (NMap.elements C_procs)
+  | None => None
+  end.
