Source/CS.v
@@ -1,0 +1,337 @@
+Require Import Common.Definitions.
+Require Import Common.Util.
+Require Import Common.Events.
+Require Import Common.Values.
+Require Import Common.Memory.
+Require Import Source.Language.
+Require Import Source.GlobalEnv.
+
+(* small-step semantics with evaluation contexts *)
+
+Inductive eval_context : Type :=
+| EC_binop_left : binop -> expr -> eval_context
+| EC_binop_right : binop -> value -> eval_context
+| EC_seq_right : expr -> eval_context
+| EC_if : expr -> expr -> eval_context
+| EC_alloc : eval_context
+| EC_deref : eval_context
+| EC_assign_right : expr -> eval_context
+| EC_assign_left : value -> eval_context
+| EC_call : Component.id -> Procedure.id -> eval_context.
+
+Definition kont : Type := list eval_context.
+Definition stack : Type := list (Component.id * value * kont).
+Definition state : Type := Component.id * stack * Memory.t * kont * expr.
+
+Inductive step (G : global_env) : state -> trace -> state -> Prop :=
+| S_binop_push_left:
+    forall C s mem ks b_op e1 e2,
+      let st := (C, s, mem, ks, E_binop b_op e1 e2) in
+      let st' := (C, s, mem, EC_binop_left b_op e2 :: ks, e1) in
+      step G st E0 st'
+| S_binop_push_right:
+    forall C s mem ks b_op v1 e2,
+      let st := (C, s, mem, EC_binop_left b_op e2 :: ks, E_val v1) in
+      let st' := (C, s, mem, EC_binop_right b_op v1 :: ks, e2) in
+      step G st E0 st'
+| S_binop_pop:
+    forall C s mem ks b_op v1 v2,
+      let st := (C, s, mem, EC_binop_right b_op v1 :: ks, E_val v2) in
+      let st' := (C, s, mem, ks, E_val (eval_binop b_op v1 v2)) in
+      step G st E0 st'
+| S_seq_push:
+    forall C s mem ks e1 e2,
+      let st := (C, s, mem, ks, E_seq e1 e2) in
+      let st' := (C, s, mem, EC_seq_right e2 :: ks, e1) in
+      step G st E0 st'
+| S_seq_pop:
+    forall C s mem ks v e2,
+      let st := (C, s, mem, EC_seq_right e2 :: ks, E_val v) in
+      let st' := (C, s, mem, ks, e2) in
+      step G st E0 st'
+| S_if_push:
+    forall C s mem ks e1 e2 e3,
+      let st := (C, s, mem, ks, E_if e1 e2 e3) in
+      let st' := (C, s, mem, EC_if e2 e3 :: ks, e1) in
+      step G st E0 st'
+| S_if_pop_conseq:
+    forall C s mem ks e2 e3 i,
+      let st := (C, s, mem, EC_if e2 e3 :: ks, E_val (Int i)) in
+      i <> 0 ->
+      let st' := (C, s, mem, ks, e2) in
+      step G st E0 st'
+| S_if_pop_alt:
+    forall C s mem ks e2 e3,
+      let st := (C, s, mem, EC_if e2 e3 :: ks, E_val (Int 0)) in
+      let st' := (C, s, mem, ks, e3) in
+      step G st E0 st'
+| S_local_buffer:
+    forall C s mem ks b,
+      let st := (C, s, mem, ks, E_local) in
+      NMap.find C (genv_buffers G) = Some b ->
+      let st' := (C, s, mem, ks, E_val (Ptr (C,b,0))) in
+      step G st E0 st'
+| S_alloc_push:
+    forall C s mem ks e,
+      let st := (C, s, mem, ks, E_alloc e) in
+      let st' := (C, s, mem, EC_alloc :: ks, e) in
+      step G st E0 st'
+| S_alloc_pop:
+    forall C s mem mem' ks size ptr,
+      let st := (C, s, mem, EC_alloc :: ks, E_val (Int size)) in
+      Memory.alloc mem C size = Some (mem', ptr) ->
+      let st' := (C, s, mem', ks, E_val (Ptr ptr)) in
+      step G st E0 st'
+| S_deref_push:
+    forall C s mem ks e,
+      let st := (C, s, mem, ks, E_deref e) in
+      let st' := (C, s, mem, EC_deref :: ks, e) in
+      step G st E0 st'
+| S_deref_pop:
+    forall C s mem ks C' b' o' v,
+      let st := (C, s, mem, EC_deref :: ks, E_val (Ptr (C',b',o'))) in
+      Memory.load mem (C',b',o') = Some v ->
+      let st' := (C, s, mem, ks, E_val v) in
+      step G st E0 st'
+| S_assign_push_arg:
+    forall C s mem ks e1 e2,
+      let st := (C, s, mem, ks, E_assign e1 e2) in
+      let st' := (C, s, mem, EC_assign_right e2 :: ks, e1) in
+      step G st E0 st'
+| S_assign_push_dest:
+    forall C s mem ks v e2,
+      let st := (C, s, mem, EC_assign_right e2 :: ks, E_val v) in
+      let st' := (C, s, mem, EC_assign_left v :: ks, e2) in
+      step G st E0 st'
+| S_assign_pop:
+    forall C s mem mem' ks v C' b' o',
+      let st := (C, s, mem, EC_assign_left v :: ks, E_val (Ptr (C',b',o'))) in
+      C = C' ->
+      Memory.store mem (C',b',o') v = Some mem' ->
+      let st' := (C, s, mem', ks, E_val v) in
+      step G st E0 st'
+| S_call_push_arg:
+    forall C s mem ks C' P e,
+      let st := (C, s, mem, ks, E_call C' P e) in
+      imported_procedure (genv_interface G) C C' P \/ C = C' ->
+      let st' := (C, s, mem, EC_call C' P :: ks, e) in
+      step G st E0 st'
+| S_call_push_proc:
+    forall C s mem mem' ks C' P v C'_procs P_expr b b' old_call_arg,
+      let st := (C, s, mem, EC_call C' P :: ks, E_val (Int v)) in
+      (* retrieve the procedure code *)
+      NMap.find C' (genv_procedures G) = Some C'_procs ->
+      NMap.find P C'_procs = Some P_expr ->
+      (* save the old call argument *)
+      NMap.find C (genv_buffers G) = Some b ->
+      Memory.load mem (C,b,0) = Some old_call_arg ->
+      (* place the call argument in the target memory *)
+      NMap.find C' (genv_buffers G) = Some b' ->
+      Memory.store mem (C',b',0) (Int v) = Some mem' ->
+      let st' := (C', (C, old_call_arg, ks) :: s, mem', [], P_expr) in
+      let t := [ECall C P v C'] in
+      step G st t st'
+| S_call_pop:
+    forall C s mem mem' ks v C' old_call_arg b,
+      let st := (C, (C',old_call_arg,ks) :: s, mem, [], E_val (Int v)) in
+      (* restore the old call argument *)
+      NMap.find C' (genv_buffers G) = Some b ->
+      Memory.store mem (C',b,0) old_call_arg = Some mem' ->
+      let st' := (C', s, mem', ks, E_val (Int v)) in
+      let t := [ERet C v C'] in
+      step G st t st'.
+
+(* functional version of step *)
+
+Definition eval_step (G : global_env) (st : state) : option (trace * state) :=
+  let '(C, s, mem, ks, e) := st in
+  match e with
+  (* pushing a new continuation *)
+  | E_binop b_op e1 e2 =>
+    Some (E0, (C, s, mem, EC_binop_left b_op e2 :: ks, e1))
+  | E_seq e1 e2 =>
+    Some (E0, (C, s, mem, EC_seq_right e2 :: ks, e1))
+  | E_if e1 e2 e3 =>
+    Some (E0, (C, s, mem, EC_if e2 e3 :: ks, e1))
+  | E_local =>
+    match NMap.find C (genv_buffers G) with
+    | Some b => Some (E0, (C, s, mem, ks, E_val (Ptr (C,b,0))))
+    | None => None
+    end
+  | E_alloc e =>
+    Some (E0, (C, s, mem, EC_alloc :: ks, e))
+  | E_deref e =>
+    Some (E0, (C, s, mem, EC_deref :: ks, e))
+  | E_assign e1 e2 =>
+    Some (E0, (C, s, mem, EC_assign_right e2 :: ks, e1))
+  | E_call C' P e =>
+    if (imported_procedure_b (genv_interface G) C C' P) || (C =? C') then
+      Some (E0, (C, s, mem, EC_call C' P :: ks, e))
+    else
+      None
+  (* evaluating current continuation *)
+  | E_val v =>
+    match ks with
+    | EC_binop_left b_op e2 :: ks' =>
+      Some (E0, (C, s, mem, EC_binop_right b_op v :: ks', e2))
+    | EC_binop_right b_op v1 :: ks' =>
+      Some (E0, (C, s, mem, ks', E_val (eval_binop b_op v1 v)))
+    | EC_seq_right e2 :: ks' =>
+      Some (E0, (C, s, mem, ks', e2))
+    | EC_if e2 e3 :: ks' =>
+      match v with
+      | Int 0 => Some (E0, (C, s, mem, ks', e3))
+      | Int i => Some (E0, (C, s, mem, ks', e2))
+      | _ => None
+      end
+    | EC_alloc :: ks' =>
+      match v with
+      | Int size =>
+        match Memory.alloc mem C size with
+        | Some (mem',ptr) => Some (E0, (C, s, mem', ks', E_val (Ptr ptr)))
+        | None => None
+        end
+      | _ => None
+      end
+    | EC_deref :: ks' =>
+      match v with
+      | Ptr (C',b',o') =>
+        match Memory.load mem (C',b',o') with
+        | Some v => Some (E0, (C, s, mem, ks', E_val v))
+        | None => None
+        end
+      | _ => None
+      end
+    | EC_assign_right e2 :: ks' =>
+      Some (E0, (C, s, mem, EC_assign_left v :: ks', e2))
+    | EC_assign_left v' :: ks' =>
+      match v with
+      | Ptr (C',b',o') =>
+        if C =? C' then
+          match Memory.store mem (C',b',o') v' with
+          | Some mem' => Some (E0, (C, s, mem', ks', E_val v'))
+          | None => None
+          end
+        else
+          None
+      | _ => None
+      end
+    | EC_call C' P :: ks' =>
+      match v with
+      | Int i =>
+        (* retrieve the procedure code *)
+        match NMap.find C' (genv_procedures G) with
+        | Some C'_procs =>
+          match NMap.find P C'_procs with
+          | Some P_expr =>
+            (* save the old call argument *)
+            match NMap.find C (genv_buffers G) with
+            | Some b =>
+              match Memory.load mem (C,b,0) with
+              | Some old_call_arg =>
+                (* place the call argument in the target memory *)
+                match NMap.find C' (genv_buffers G) with
+                | Some b' =>
+                  match Memory.store mem (C',b',0) (Int i) with
+                  | Some mem' =>
+                    let t := [ECall C P i C'] in
+                    Some (t, (C', (C, old_call_arg, ks') :: s, mem', [], P_expr))
+                  | None => None
+                  end
+                | None => None
+                end
+              | None => None
+              end
+            | None => None
+            end
+          | None => None
+          end
+        | None => None
+        end
+      | _ => None
+      end
+    | [] =>
+      match v, s with
+      | Int i, (C',old_call_arg,ks) :: s' =>
+        (* restore the old call argument *)
+        match NMap.find C' (genv_buffers G) with
+        | Some b =>
+          match Memory.store mem (C',b,0) old_call_arg with
+          | Some mem' =>
+            let t := [ERet C i C'] in
+            Some (t, (C', s', mem', ks, E_val (Int i)))
+          | None => None
+          end
+        | None => None
+        end
+      | _, _ => None
+      end
+    end
+  | _ => None
+  end.
+
+Theorem step_implies_eval_step:
+  forall G st t st',
+    step G st t st' -> eval_step G st =  Some (t, st').
+Proof.
+  intros G st t st' Hstep.
+  inversion Hstep; subst; simpl; auto.
+  (* if expressions *)
+  - apply beq_nat_false_iff in H.
+    destruct i eqn:Hi; auto.
+    + inversion H.
+  (* local buffers *)
+  - rewrite H. auto.
+  (* memory allocs *)
+  - rewrite H. auto.
+  (* memory loads *)
+  - unfold Memory.load in H.
+    destruct (NMap.find (elt:=ComponentMemory.t) C' mem) eqn:HC'mem.
+    + rewrite H. auto.
+    + inversion H.
+  (* memory stores *)
+  - rewrite <- beq_nat_refl.
+    unfold Memory.store in H0.
+    destruct (NMap.find (elt:=ComponentMemory.t) C' mem) eqn:HC'mem.
+    + rewrite H0. auto.
+    + inversion H0.
+  (* calls/returns *)
+  - destruct H.
+    + destruct H as [CI [HCI Himport]].
+      unfold Program.has_component in HCI.
+      unfold Component.is_importing in Himport.
+      unfold imported_procedure_b.
+      apply NMap.find_1 in HCI. rewrite HCI.
+      rewrite count_occ_In in Himport.
+      inversion Himport.
+      * rewrite <- H0. simpl. auto.
+      * rewrite <- H. simpl. auto.
+    + unfold st'0. rewrite H. rewrite <- beq_nat_refl.
+      rewrite orb_true_r. auto.
+  - rewrite H, H0, H1, H3.
+    unfold Memory.load in H2.
+    destruct (NMap.find (elt:=ComponentMemory.t) C mem) eqn:HCmem.
+    + rewrite H2.
+      unfold Memory.store in H4.
+      destruct (NMap.find (elt:=ComponentMemory.t) C' mem) eqn:HC'mem.
+      * inversion HCmem. subst. rewrite H4. auto.
+      * inversion H4.
+    + inversion H2.
+  - rewrite H.
+    unfold Memory.store in H0.
+    destruct (NMap.find (elt:=ComponentMemory.t) C' mem) eqn:HC'mem.
+    + rewrite H0. auto.
+    + inversion H0.
+Qed.
+
+Theorem step_determinism:
+  forall G st t st1 st2,
+    step G st t st1 -> step G st t st2 -> st1 = st2.
+Proof.
+  intros G st t st1 st2 Hstep1 Hstep2.
+  apply step_implies_eval_step in Hstep1.
+  apply step_implies_eval_step in Hstep2.
+  rewrite Hstep1 in Hstep2.
+  inversion Hstep2.
+  auto.
+Qed.
