Source/GlobalEnv.v
@@ -1,0 +1,9 @@
+Require Import Common.Definitions.
+Require Import Common.Values.
+Require Import Source.Language.
+
+Record global_env : Type := mkGlobalEnv {
+  genv_interface : Program.interface;
+  genv_procedures : NMap.t (NMap.t expr);
+  genv_buffers : NMap.t Block.id
+}.
