Source/Language.v
@@ -1,0 +1,21 @@
+Require Import Common.Definitions.
+Require Import Common.Values.
+Require Import Common.Memory.
+
+Inductive expr : Type :=
+| E_val : value -> expr
+| E_local : expr
+| E_binop : binop -> expr -> expr -> expr
+| E_seq : expr -> expr -> expr
+| E_if : expr -> expr -> expr -> expr
+| E_alloc : expr -> expr
+| E_deref : expr -> expr
+| E_assign : expr -> expr -> expr
+| E_call : Component.id -> Procedure.id -> expr -> expr
+| E_exit : expr.
+
+Record program : Type := mkProg {
+  prog_interface : Program.interface;
+  prog_procedures : NMap.t (NMap.t expr);
+  prog_buffers : NMap.t nat
+}.
